src/named/egraph/UFProofs.v
@@ -1,0 +1,1317 @@
+Set Implicit Arguments.
+Set Bullet Behavior "Strict Subproofs".
+
+Require Import NArith List.
+Import ListNotations.
+Open Scope list.
+
+Require Import Tries.Canonical.
+Import PTree.
+
+From Utils Require Import Utils Monad.
+From Named Require Import Core.
+Import Core.Notations.
+
+
+Require Import Utils.UnionFind.
+Require Import Utils.TrieMap.
+Import TrieArrayList.
+From coqutil Require Import Map.Interface.
+
+Section WithVar.
+  Context (V : Type)
+          {V_Eqb : Eqb V}
+          {V_default : WithDefault V}.
+
+  Notation named_list := (@named_list V).
+  Notation named_map := (@named_map V).
+  Notation term := (@term V).
+  Notation ctx := (@ctx V).
+  Notation sort := (@sort V).
+  Notation subst := (@subst V).
+  Notation rule := (@rule V).
+  Notation lang := (@lang V).
+  
+  Notation eq_subst l :=
+    (eq_subst (Model:= core_model l)).
+  Notation eq_args l :=
+    (eq_args (Model:= core_model l)).
+  Notation wf_subst l :=
+    (wf_subst (Model:= core_model l)).
+  Notation wf_args l :=
+    (wf_args (Model:= core_model l)).
+  Notation wf_ctx l :=
+    (wf_ctx (Model:= core_model l)).
+
+  Variant node : Type :=
+    (* variable name *)
+    | nvar : V -> node
+    (* Rule label, list of subterms*)
+    | ncon : V -> list positive -> node.
+                                     (*
+    | ncemp : node
+    | nccons : positive -> positive -> node.*)
+
+  (* We assume that the head is the root by default.
+     Invariant: all indices of the head are < length of the tail
+   *)
+
+  Definition pf := list node.
+
+  (*TODO: backport these to core.v. Copied from TreeProofs.v*)
+    
+    Local Lemma term_con_congruence l c t name s1 s2 c' args t'
+      : In (name, term_rule c' args t') l ->
+        t = t'[/with_names_from c' s2/] ->
+        wf_lang l ->
+        eq_args l c c' s1 s2 ->
+        eq_term l c t (con name s1) (con name s2).
+    Proof.
+      intros.
+      assert (wf_ctx l c') by with_rule_in_wf_crush.
+      rewrite <- (wf_con_id_args_subst c' s1);[| basic_core_crush..].
+      rewrite <- (wf_con_id_args_subst c' s2);[|basic_core_crush..].
+      subst.
+      change (con ?n ?args[/?s/]) with (con n args)[/s/].
+      eapply eq_term_subst; eauto.
+      {
+        apply eq_args_implies_eq_subst; eauto.
+      }
+      {
+        constructor.
+        replace t' with t'[/id_subst c'/].
+        - eapply wf_term_by; basic_core_crush.
+        - basic_core_crush.
+      }
+    Qed.
+
+    
+    Local Lemma sort_con_congruence l c name s1 s2 c' args
+      : In (name, sort_rule c' args) l ->
+        wf_lang l ->
+        eq_args l c c' s1 s2 ->
+        eq_sort l c (scon name s1) (scon name s2).
+    Proof.
+      intros.
+      assert (wf_ctx l c') by with_rule_in_wf_crush.
+      rewrite <- (wf_con_id_args_subst c' s1);[| basic_core_crush..].
+      rewrite <- (wf_con_id_args_subst c' s2);[|basic_core_crush..].
+      subst.
+      change (scon ?n ?args[/?s/]) with (scon n args)[/s/].
+      eapply eq_sort_subst; eauto.
+      { apply eq_args_implies_eq_subst; eauto. }
+      { constructor.
+        eapply wf_sort_by; basic_core_crush.
+      }
+    Qed.
+
+  
+    
+  
+  Section WithLang.
+
+    Context (l : lang).
+
+
+  Fixpoint named_list_put {A B} `{Eqb A} (l : @Utils.named_list A B) k v :=
+    match l with
+    | [] => [(k,v)]
+    | (k',v')::l =>
+        if eqb k k' then (k,v)::l else (k',v')::(named_list_put l k v)
+    end.
+
+  Fixpoint named_list_remove {A B} `{Eqb A} (l : @Utils.named_list A B) k :=
+    match l with
+    | [] => []
+    | (k',v')::l =>
+        if eqb k k' then l else (k',v')::(named_list_remove l k)
+    end.
+
+
+        
+    (*TODO: copied; should be deduplicated if not replaced *)
+  Section __.
+    (* Not fast, but will run*)
+    Local Instance named_list_map A B `{Eqb A} : map.map A B :=
+      {
+        rep := @Utils.named_list A B;
+        get := named_list_lookup_err;
+        empty := [];
+        put := named_list_put;
+        remove := named_list_remove;
+        fold _ f acc l := List.fold_left (fun acc '(k, v) => f acc k v) l acc;
+      }.
+  End __.
+
+  (*TODO: this isn't very efficient*)
+
+  Axiom eqb_node : Eqb node.
+  Existing Instance eqb_node.
+  Definition node_map := (@named_list_map node positive _).
+
+  (* Basically an egraph without congruence closure or saturation *)
+  Record proof_context :=
+    MkPC {
+        id_equiv :  union_find;
+        hashcons : node_map;
+      }.
+
+  Import StateMonad.
+
+  Notation pfM := (stateT proof_context option).
+
+  (*TODO: move to Monad.v*)
+  
+Notation "'let' p <^- e 'in' b" :=
+  (Mbind (fun p => b) (lift e))
+    (in custom monadic_do at level 200, left associativity, p pattern at level 0, e constr, b custom monadic_do).
+
+
+  Notation "'ret' { M } e" := (Mret (M:=M) e) (in custom monadic_do at level 90, e constr).
+
+Notation "'let' { M } p <- e 'in' b" :=
+  (Mbind (M:=M) (fun p => b) e)
+    (in custom monadic_do at level 200, left associativity, p pattern at level 0, e constr, b custom monadic_do).
+
+Notation "'let' { M } p <?- e 'in' b" :=
+  (Mbind (M:=M) (fun x => match x with p => b | _ => default end) e)
+    (in custom monadic_do at level 200, left associativity, p pattern at level 0, e constr, b custom monadic_do).
+
+Instance stateT_default S M A `{WithDefault (M (A*S))%type}
+  : WithDefault (stateT S M A) :=
+  fun _ => default.
+
+Existing  Instance stateT_trans.
+  
+  Definition find i : pfM positive :=
+    fun pc =>
+      @! let (uf', i') <- find pc.(id_equiv) i in
+        ret (i',MkPC uf' pc.(hashcons)).
+
+  
+  Definition alloc : pfM positive :=
+    fun pc => let (uf', i') := alloc pc.(id_equiv) in
+              Some (i', MkPC uf' pc.(hashcons)).
+
+  
+  Definition set_hashcons n i : pfM unit :=
+    fun pc => let hc' := map.put pc.(hashcons) n i in
+              Some (tt, MkPC pc.(id_equiv) hc').
+
+  Definition canonicalize n : pfM node :=
+    match n with     
+    | ncon name args =>
+        @! let args <- list_Mmap find args in       
+          ret ncon name args
+    | nvar x =>
+        @! ret nvar x
+    end.
+
+    
+    Definition eqb_ids a b : pfM unit :=
+      @! let fa <- (find a) in
+         let fb <- (find b) in
+         let ! eqb fa fb in
+         ret tt.
+
+    (*TODO: what's the right output type?
+      Shouldn't need the 2nd option (but then need a different combinator)
+     *)
+    Definition lookup n : pfM (option positive) :=
+      fun pc =>
+        let mi := map.get pc.(hashcons) n in
+        Some (mi,pc).
+  
+      (*
+      Adds a node to the egraph without checking whether it is valid in the language
+     *)
+    Definition add_node_unchecked (n : node) : pfM positive :=
+      @! let mn <- lookup n in
+         match mn with
+         | Some i => @! ret i
+         | None => 
+             @! let i <- alloc in
+                let tt <- set_hashcons n i in
+                ret i
+         end.
+
+    
+    Fixpoint lookup_term (pc : proof_context) (e : term) : option _ :=
+      match e with
+      | var x => map.get pc.(hashcons) (nvar x)
+      | con n s =>
+          @! let si <- list_Mmap (lookup_term pc) s in
+            (map.get pc.(hashcons) (ncon n si))
+      end.
+
+    Definition lookup_sort (pc : proof_context) (t : sort) : option _ :=
+      match t with
+      | scon n s =>
+          @! let si <- list_Mmap (lookup_term pc) s in
+            (map.get pc.(hashcons) (ncon n si))
+      end.
+    
+
+    Section UnderSubst.
+      
+      Context (sub : named_list positive).
+
+      
+      Fixpoint lookup_term' (pc : proof_context) (e : term) : option _ :=
+        match e with
+        | var x => (named_list_lookup_err sub x)
+        | con n s =>
+            @! let si <- list_Mmap (lookup_term' pc) s in
+              (map.get pc.(hashcons) (ncon n si))
+        end.
+
+      Definition lookup_sort' (pc : proof_context) (t : sort) : option _ :=
+        match t with
+        | scon n s =>
+            @! let si <- list_Mmap (lookup_term' pc) s in
+              (map.get pc.(hashcons) (ncon n si))
+        end.
+
+      Fixpoint add_term_unchecked' (e : term) {struct e} : pfM positive :=
+        match e with
+        | var x => lift (named_list_lookup_err sub x)
+        | con n s =>
+            @! let si  <- list_Mmap add_term_unchecked' s in
+              (add_node_unchecked (ncon n si))
+        end.
+      
+      Definition add_sort_unchecked' (t: sort) : pfM positive :=
+        match t with
+        | scon n s =>
+            @! let si <- list_Mmap add_term_unchecked' s in
+              (add_node_unchecked (ncon n si))
+        end.
+
+    End UnderSubst.
+
+    (*
+
+               
+     Fixpoint add_term_unchecked (e : term) {struct e} : pfM positive :=
+        match e with
+        | var x => add_node_unchecked (nvar x)
+        | con n s =>
+            @! let si  <- list_Mmap add_term_unchecked s in
+               (add_node_unchecked (ncon n si))
+        end.
+      
+      Definition add_sort_unchecked (t: sort) : pfM positive :=
+        match t with
+        | scon n s =>
+            @! let si <- list_Mmap add_term_unchecked s in
+               (add_node_unchecked (ncon n si))
+        end.
+
+    *)
+    
+    (*
+  Section WithCtx.
+    (*TODO: ids or sorts on rhs*)
+    Context (c : named_list positive).*)
+      
+      Section Inner.
+
+        (*TODO: return sort or no?*)
+        Context (add_term' : term -> (*sort*) positive-> pfM positive).
+
+        (*TODO: return pair of lists or list of pairs?*)
+        Fixpoint add_args' (s : list term) (c : ctx) {struct s}
+          : pfM (list positive) :=
+          match s, c with
+          | [],[] => @! ret []
+          | e::s, (_,t)::c =>
+              @! let sci <- add_args' s c in
+                (* sort given by c *)
+                let ti <- add_sort_unchecked' (with_names_from c sci) t in
+                let ei <- add_term' e ti in
+                (*  let tt <- eqb_ids ti' ti in *)
+                ret ei::sci
+          | _,_ => default
+          end.
+      End Inner.
+
+      Section UnderSubst.
+      
+        Context (sub : named_list positive).
+        
+        Fixpoint add_term' (e : term) (t_in : positive) {struct e} : pfM positive :=
+          match e with
+          | var x => lift (named_list_lookup_err sub x)
+          | con n s =>
+              @! let term_rule c _ t <?- lift (named_list_lookup_err l n) in
+                let sci <- add_args' add_term' s c in
+                (* sort generated from sort of n rule *)
+                let t_out <- add_sort_unchecked' (with_names_from c sci) t in
+                let tt <- eqb_ids t_in t_out in
+                (add_node_unchecked (ncon n sci))
+          end.
+
+        Definition add_sort' (t : sort) : pfM positive :=
+          let (n,s) := t in
+          @! let sort_rule c _ <?- lift (named_list_lookup_err l n) in
+            let sci <- add_args' add_term' s c in
+            (add_node_unchecked (ncon n sci)).
+            
+      End UnderSubst.
+
+      Section WithCtx.
+      
+        Context (ctx : named_list positive).
+      
+        
+        Fixpoint add_term (e : term) (t_in : positive) {struct e} : pfM positive :=
+          match e with
+          | var x =>
+              @! let t_out <^- (named_list_lookup_err ctx x) in
+                let tt <- eqb_ids t_in t_out in
+                (add_node_unchecked (nvar x))
+          | con n s =>
+              @! let term_rule c _ t <?- lift (named_list_lookup_err l n) in
+                let sci <- add_args' add_term s c in
+                (* sort generated from sort of n rule *)
+                let t_out <- add_sort_unchecked' (with_names_from c sci) t in
+                let tt <- eqb_ids t_in t_out in
+                (add_node_unchecked (ncon n sci))
+          end.
+
+        Definition add_sort (t : sort) : pfM positive :=
+          let (n,s) := t in
+          @! let sort_rule c _ <?- lift (named_list_lookup_err l n) in
+            let sci <- add_args' add_term s c in
+            (add_node_unchecked (ncon n sci)).
+            
+      End WithCtx.
+
+      Section WithCtx.
+        Context (c : ctx).
+
+        
+        Definition lookup_sort_of_node (pc : proof_context) (n : node)
+          : option _ :=
+          match n with
+          | nvar x =>
+              @!let t <- named_list_lookup_err c x in
+              (*TODO: do I want to have this precomputed?*)
+                (lookup_sort pc t)
+          | ncon n s =>
+              @! let (term_rule _ _ t) <?- named_list_lookup_err l n in
+                (lookup_sort' (with_names_from c s) pc t)
+          end.
+  
+        
+        Definition lookup_term_and_sort (pc : proof_context) (e : term)
+          : option _ :=
+          match e with
+          | var x =>
+              @! let i <- map.get pc.(hashcons) (nvar x) in
+                let ti <- lookup_sort_of_node pc (nvar x) in
+                ret (i,ti)
+          | con n s =>
+              @! let si <- list_Mmap (lookup_term pc) s in
+                let i <- map.get pc.(hashcons) (ncon n si) in
+                let ti <- lookup_sort_of_node pc (ncon n si) in
+                ret (i,ti)
+          end.
+
+        (*TODO: is R really right?*)
+      Definition proof_context_valid pc t :=
+        uf_ok pc.(id_equiv) t
+                  /\ (forall i t, Some i = lookup_sort pc t -> wf_sort l c t)
+                  /\ (forall ti i e t,
+                         Some ti = lookup_sort pc t ->
+                         Some (i,ti) = lookup_term_and_sort pc e ->
+                         wf_term l c e t).
+
+      Definition empty := MkPC empty map.empty.
+
+      Lemma empty_ok
+        : proof_context_valid empty [].
+      Proof.
+        unfold proof_context_valid.
+        split.
+        {
+          apply empty_ok.
+        }
+        split.
+        all:intros; simpl in *.
+        {
+          destruct t0; simpl in *.
+          revert H; case_match; congruence.
+        }
+        {
+          destruct e; simpl in *; try congruence.
+          revert H0; case_match; congruence.
+        }
+      Qed.
+
+      
+      Lemma lookup_term_forest_equiv f f' pc1 pc2 e
+        : forest_equiv f f' ->
+          uf_ok pc1.(id_equiv) f ->
+          uf_ok pc2.(id_equiv) f' ->
+          pc1.(hashcons) = pc2.(hashcons) ->
+          lookup_term pc1 e = lookup_term pc2 e.
+      Proof.
+        intros; induction e;
+          intros; simpl in *.
+        1: destruct pc1; destruct pc2; simpl in *; subst; now auto.
+        enough (list_Mmap (lookup_term pc1) l0
+                = list_Mmap (lookup_term pc2) l0) as H'
+            by (rewrite H'; case_match; congruence).
+        revert dependent l0.
+        induction l0;
+          intros; simpl in *; auto.
+        break.
+        rewrite H3.
+        case_match; auto.
+        rewrite IHl0; eauto.
+      Qed.
+
+      (* TODO: generalize*)
+      Lemma list_Mmap_ext_option {A B} (f g : A -> option B) ls
+        : (forall x, f x = g x) -> list_Mmap f ls = list_Mmap g ls.
+      Proof.
+        intro; induction ls;
+          basic_goal_prep;
+          basic_utils_crush.
+        rewrite H.
+        case_match; auto.
+        rewrite IHls.
+        case_match; auto.
+      Qed.
+      
+      Lemma map_lookup_term_forest_equiv f f' pc1 pc2 e
+        : forest_equiv f f' ->
+          uf_ok pc1.(id_equiv) f ->
+          uf_ok pc2.(id_equiv) f' ->
+          pc1.(hashcons) = pc2.(hashcons) ->
+          list_Mmap (lookup_term pc1) e = list_Mmap (lookup_term pc2) e.
+      Proof.
+        intros; eapply list_Mmap_ext_option.
+        intros; eapply lookup_term_forest_equiv; eauto.
+      Qed.
+        
+      Lemma lookup_sort_forest_equiv f f' pc1 pc2 t
+        : forest_equiv f f' ->
+          uf_ok pc1.(id_equiv) f ->
+          uf_ok pc2.(id_equiv) f' ->
+          pc1.(hashcons) = pc2.(hashcons) ->
+          lookup_sort pc1 t = lookup_sort pc2 t.
+      Proof.
+        intros; induction t;
+          intros; simpl in *.
+        enough (list_Mmap (lookup_term pc1) l0
+                = list_Mmap (lookup_term pc2) l0) as H'
+            by (rewrite H'; case_match; congruence).
+        eapply map_lookup_term_forest_equiv; eauto.
+      Qed.
+
+      
+      Lemma lookup_term'_forest_equiv f f' pc1 pc2 e sub
+        : forest_equiv f f' ->
+          uf_ok pc1.(id_equiv) f ->
+          uf_ok pc2.(id_equiv) f' ->
+          pc1.(hashcons) = pc2.(hashcons) ->
+          lookup_term' sub pc1 e = lookup_term' sub pc2 e.
+      Proof.
+        intros; induction e;
+          intros; simpl in *.
+        1: destruct pc1; destruct pc2; simpl in *; subst; now auto.
+        enough (list_Mmap (lookup_term' sub pc1) l0
+                = list_Mmap (lookup_term' sub pc2) l0) as H'
+            by (rewrite H'; case_match; congruence).
+        revert dependent l0.
+        induction l0;
+          intros; simpl in *; auto.
+        break.
+        rewrite H3.
+        case_match; auto.
+        rewrite IHl0; eauto.
+      Qed.
+      
+      Lemma map_lookup_term'_forest_equiv f f' pc1 pc2 e sub
+        : forest_equiv f f' ->
+          uf_ok pc1.(id_equiv) f ->
+          uf_ok pc2.(id_equiv) f' ->
+          pc1.(hashcons) = pc2.(hashcons) ->
+          list_Mmap (lookup_term' sub pc1) e = list_Mmap (lookup_term' sub pc2) e.
+      Proof.
+        intros; eapply list_Mmap_ext_option.
+        intros; eapply lookup_term'_forest_equiv; eauto.
+      Qed.
+        
+
+      
+      Lemma lookup_sort'_forest_equiv f f' pc1 pc2 t sub
+        : forest_equiv f f' ->
+          uf_ok pc1.(id_equiv) f ->
+          uf_ok pc2.(id_equiv) f' ->
+          pc1.(hashcons) = pc2.(hashcons) ->
+          lookup_sort' sub pc1 t = lookup_sort' sub pc2 t.
+      Proof.
+        intros; induction t;
+          intros; simpl in *.
+        enough (list_Mmap (lookup_term' sub pc1) l0
+                = list_Mmap (lookup_term' sub pc2) l0) as H'
+            by (rewrite H'; case_match; congruence).
+        eapply map_lookup_term'_forest_equiv; eauto.
+      Qed.
+
+      
+        
+      Lemma lookup_term_and_sort_forest_equiv f f' pc1 pc2 e
+        : forest_equiv f f' ->
+          uf_ok pc1.(id_equiv) f ->
+          uf_ok pc2.(id_equiv) f' ->
+          pc1.(hashcons) = pc2.(hashcons) ->
+          lookup_term_and_sort pc1 e = lookup_term_and_sort pc2 e.
+      Proof.
+        intros; induction e;
+          intros; simpl in *.
+        {
+          destruct pc1; destruct pc2; simpl in *; subst.
+          case_match; eauto.
+          my_case Heqnl (named_list_lookup_err c n); eauto.
+          erewrite lookup_sort_forest_equiv; eauto.
+        }
+        {
+          erewrite map_lookup_term_forest_equiv; eauto.
+          case_match; eauto.
+          rewrite H2; case_match; eauto.
+          my_case Hnl (named_list_lookup_err l n); auto.
+          my_case Hr r; eauto.
+          erewrite lookup_sort'_forest_equiv; eauto.
+        }
+      Qed.
+
+      
+      Lemma lookup_term_forest_subrel f f' pc1 pc2 e
+        : forest_subrel f f' ->
+          uf_ok pc1.(id_equiv) f ->
+          uf_ok pc2.(id_equiv) f' ->
+          pc1.(hashcons) = pc2.(hashcons) ->
+          forall i,
+            Some i = lookup_term pc1 e ->
+            Some i = lookup_term pc2 e.
+      Proof.
+        intros Hsub Hokf Hokf';
+          induction e;
+          intros; simpl in *.
+        1: destruct pc1; destruct pc2; simpl in *; subst; now auto.
+        revert H1; 
+          case_match;[| congruence].
+        
+        enough (Some l1 = list_Mmap (lookup_term pc2) l0) as H'.
+        {
+          rewrite<- H'.
+          congruence.
+        }
+        revert dependent l1.
+        revert dependent l0.
+        induction l0;
+          intros; simpl in *; auto.
+        break.
+        revert HeqH1.
+        case_match;[| congruence].
+        case_match;[| congruence].
+        intro H'; safe_invert H'.
+        specialize (H H0 p eq_refl).
+        rewrite <- H.
+        erewrite <- IHl0; eauto.
+      Qed.
+      
+      Lemma map_lookup_term_forest_subrel f f' pc1 pc2 e
+        : forest_subrel f f' ->
+          uf_ok pc1.(id_equiv) f ->
+          uf_ok pc2.(id_equiv) f' ->
+          pc1.(hashcons) = pc2.(hashcons) ->
+          forall l,
+            Some l = list_Mmap (lookup_term pc1) e ->
+            Some l = list_Mmap (lookup_term pc2) e.
+      Proof.
+        intros ? ? ? ?.
+        induction e;
+          intros; simpl in *; auto.
+        break.
+        revert H3.
+        case_match;[| congruence].
+        case_match;[| congruence].
+        intro H'; safe_invert H'.
+        erewrite <- lookup_term_forest_subrel; eauto.
+        erewrite <- IHe; eauto.
+      Qed.
+
+      Lemma lookup_sort_forest_subrel f f' pc1 pc2 t
+        : forest_subrel f f' ->
+          uf_ok pc1.(id_equiv) f ->
+          uf_ok pc2.(id_equiv) f' ->
+          pc1.(hashcons) = pc2.(hashcons) ->
+          forall i,
+            Some i = lookup_sort pc1 t ->
+            Some i = lookup_sort pc2 t.
+      Proof.
+        
+        intros Hsub Hokf Hokf';
+          induction t;
+          intros; simpl in *.
+        revert H0; 
+          case_match;[| congruence].
+        
+        enough (Some l1 = list_Mmap (lookup_term pc2) l0) as H'.
+        {
+          rewrite<- H'.
+          congruence.
+        }
+        revert dependent l1.
+        revert dependent l0.
+        induction l0;
+          intros; simpl in *; auto.
+        break.
+        revert HeqH0.
+        case_match;[| congruence].
+        case_match;[| congruence].
+        intro H'; safe_invert H'.
+        erewrite <- lookup_term_forest_subrel; eauto.
+        erewrite <- IHl0; eauto.
+      Qed.
+
+      (*TODO: concerning; why is this true?*)
+      Lemma lookup_term'_forest_subrel f f' pc1 pc2 e sub
+        : forest_subrel f f' ->
+          uf_ok pc1.(id_equiv) f ->
+          uf_ok pc2.(id_equiv) f' ->
+          pc1.(hashcons) = pc2.(hashcons) ->
+          lookup_term' sub pc1 e = lookup_term' sub pc2 e.
+      Proof.
+        intros; induction e;
+          intros; simpl in *.
+        1: destruct pc1; destruct pc2; simpl in *; subst; now auto.
+        enough (list_Mmap (lookup_term' sub pc1) l0
+                = list_Mmap (lookup_term' sub pc2) l0) as H'
+            by (rewrite H'; case_match; congruence).
+        revert dependent l0.
+        induction l0;
+          intros; simpl in *; auto.
+        break.
+        rewrite H3.
+        case_match; auto.
+        rewrite IHl0; eauto.
+      Qed.
+      
+      Lemma map_lookup_term'_forest_subrel f f' pc1 pc2 e sub
+        : forest_subrel f f' ->
+          uf_ok pc1.(id_equiv) f ->
+          uf_ok pc2.(id_equiv) f' ->
+          pc1.(hashcons) = pc2.(hashcons) ->
+          list_Mmap (lookup_term' sub pc1) e = list_Mmap (lookup_term' sub pc2) e.
+      Proof.
+        intros; eapply list_Mmap_ext_option.
+        intros; eapply lookup_term'_forest_subrel; eauto.
+      Qed.
+        
+
+      
+      Lemma lookup_sort'_forest_subrel f f' pc1 pc2 t sub
+        : forest_subrel f f' ->
+          uf_ok pc1.(id_equiv) f ->
+          uf_ok pc2.(id_equiv) f' ->
+          pc1.(hashcons) = pc2.(hashcons) ->
+          lookup_sort' sub pc1 t = lookup_sort' sub pc2 t.
+      Proof.
+        intros; induction t;
+          intros; simpl in *.
+        enough (list_Mmap (lookup_term' sub pc1) l0
+                = list_Mmap (lookup_term' sub pc2) l0) as H'
+            by (rewrite H'; case_match; congruence).
+        eapply map_lookup_term'_forest_subrel; eauto.
+      Qed.
+
+      
+        
+      Lemma lookup_term_and_sort_forest_subrel f f' pc1 pc2 e
+        : forest_subrel f f' ->
+          uf_ok pc1.(id_equiv) f ->
+          uf_ok pc2.(id_equiv) f' ->
+          pc1.(hashcons) = pc2.(hashcons) ->
+          forall p,
+          Some p = lookup_term_and_sort pc1 e ->
+          Some p = lookup_term_and_sort pc2 e.
+      Proof.
+        intros ? ? ? ?; induction e;
+          intros; simpl in *.
+        {
+          revert H3.
+          destruct pc1; destruct pc2; simpl in *; subst.
+          case_match; eauto.
+          my_case Heqnl (named_list_lookup_err c n); eauto.
+          case_match; [|congruence].
+          erewrite <- lookup_sort_forest_subrel; cycle 5;
+          eauto.
+        }
+        {
+          revert H4.
+          case_match; [|congruence].
+          erewrite <- map_lookup_term_forest_subrel; cycle 5; eauto.
+          rewrite H2; case_match; eauto.
+          my_case Hnl (named_list_lookup_err l n); auto.
+          my_case Hr r; eauto.
+          erewrite lookup_sort'_forest_subrel; eauto.
+        }
+      Qed.
+        
+
+      Lemma find_ok pc f pc' (i i' : positive)
+        : proof_context_valid pc f ->
+          Some (i', pc') = find i pc ->
+          equiv_by_forest f i i'
+          /\ (exists f', forest_equiv f f' /\ proof_context_valid pc' f').
+      Proof.
+        unfold proof_context_valid.
+        intros; break.
+        revert H0; unfold find.
+        destruct pc.
+        simpl in *.
+        case_match; try congruence.
+        break.
+        intro H'; safe_invert H'.
+        eapply find_spec in HeqH0; eauto; break.
+        intuition subst.
+        eexists; intuition eauto.
+        {
+          eapply H1; eauto.
+          erewrite lookup_sort_forest_equiv; eauto.
+        }
+        {
+          eapply H2; eauto.
+          -erewrite lookup_sort_forest_equiv; eauto.
+          -erewrite lookup_term_and_sort_forest_equiv; eauto.
+        }
+      Qed.
+
+      Definition union i1 i2 : pfM positive :=
+        fun pc =>
+          @! let (uf', i') <- union pc.(id_equiv) i1 i2 in
+            ret (i',MkPC uf' pc.(hashcons)).
+      
+      Lemma union_ok pc f pc' i' (i1 i2 : positive)
+        : proof_context_valid pc f ->
+          Some (i', pc') = union i1 i2 pc ->
+          exists f', forest_subrel f f'
+                     /\ equiv_by_forest f' i1 i'
+                     /\ equiv_by_forest f' i2 i'
+                     /\ proof_context_valid pc' f'.
+      Proof.
+        unfold union.
+        intro.
+        destruct pc; simpl in *.
+        case_match; try congruence.
+        break.
+        intro H'; safe_invert H'.
+        revert HeqH0.
+        intro.
+        destruct H; simpl in *.
+        eapply union_spec in HeqH0; eauto.
+        break.
+        eexists; intuition eauto.
+        constructor; intuition eauto.
+        {
+          eapply H0.
+          eapply lookup_sort_forest_subrel; cycle 4.
+          1:eauto.
+          all:simpl.
+          2:eauto.
+          2:eauto.
+          2:eauto.
+          TODO: need better spec for union;
+          need to know it's the least rel that satisfies conditions
+          TODO: subrel in the wrong direction
+          TODO: uf_ok not true
+          eapply lookup_term_and_sort_forest_subrel .
+          TODO: need rewrite subrel
+          erewrite lookup_sort_forest_equiv; eauto.
+          admit (*lemma*).
+        }
+        {
+          eapply H1.
+          1: erewrite  lookup_sort_forest_equiv; eauto.
+          1:admit (*lemma*).
+          erewrite lookup_term_and_sort_forest_equiv; eauto.
+          admit (*lemma*).
+        }
+        {
+          
+        }
+        4: constructor; eauto.
+        1:
+        
+        unfold UnionFind.union.
+        simpl.
+        destruct H.
+        case_match; try congruence.
+        break.
+        eapply find_spec in HeqH1; eauto.
+        case_match; try congruence.
+        break.
+        eapply find_spec in HeqH2; eauto.
+        (*TODO: copied*)
+        
+        Ltac destruct_pos_eqb i j :=
+          let Hneq := fresh "Hneq" in
+          let Hneq' := fresh "Hneq" in
+          destruct (Pos.eq_dec i j) as [? | Hneq];
+          [ subst; rewrite Pos.eqb_refl
+          | pose proof Hneq as Hneq'; apply Pos.eqb_neq in Hneq'; rewrite Hneq'].
+        destruct_pos_eqb p0 p1.
+        {
+          intro H'; safe_invert H'.
+          break.
+          eexists; intuition eauto.
+          1:admit (*lemma*).
+          1:admit (*lemma *).
+          constructor; simpl; eauto.
+          1:admit (*lemma*).
+          split.
+          all: intros.
+          {
+            eapply H0.
+            erewrite  lookup_sort_forest_equiv; eauto.
+            admit (*lemma*).
+          }
+          {
+            eapply H1.
+            1: erewrite  lookup_sort_forest_equiv; eauto.
+            1:admit (*lemma*).
+            erewrite lookup_term_and_sort_forest_equiv; eauto.
+            admit (*lemma*).
+          }
+        }
+        {
+          case_match;[| congruence].
+          case_match;[| congruence].
+          destruct (PeanoNat.Nat.compare_spec n0 n).
+          all: intro H'; safe_invert H'.
+          all: break.
+          case_match;[| congruence].
+          
+        }
+        
+
+  Section WithProofCtx.
+    Context (pc : proof_context).
+
+    (*TODO: make i the canonical node*)
+    Definition node_at n i :=      
+      Some i = map.get pc.(hashcons) n.
+
+     (*
+  Inductive eq_sort : ctx -> sort -> sort -> Prop :=
+  | eq_sort_by : forall c name t1 t2,
+      In (name, sort_eq_rule c t1 t2) l ->
+      eq_sort c t1 t2
+  | eq_sort_subst : forall c s1 s2 c' t1' t2',
+      (* Need to assert wf_ctx c here to satisfy
+         assumptions' presuppositions
+       *)
+      wf_ctx c' ->
+      eq_subst (Model:= mut_mod eq_sort eq_term wf_sort wf_term) c c' s1 s2 ->
+      eq_sort c' t1' t2' ->
+      eq_sort c t1'[/s1/] t2'[/s2/]
+  | eq_sort_refl : forall c t,
+      wf_sort c t ->
+      eq_sort c t t
+  | eq_sort_trans : forall c t1 t12 t2,
+      eq_sort c t1 t12 ->
+      eq_sort c t12 t2 ->
+      eq_sort c t1 t2
+  | eq_sort_sym : forall c t1 t2, eq_sort c t1 t2 -> eq_sort c t2 t1
+  with eq_term : ctx -> sort -> term -> term -> Prop :=
+  | eq_term_subst : forall c s1 s2 c' t e1 e2,
+      (* Need to assert wf_ctx c' here to satisfy
+         assumptions' presuppositions
+       *)
+      wf_ctx c' ->
+      eq_subst (Model:= mut_mod eq_sort eq_term wf_sort wf_term) c c' s1 s2 ->
+      eq_term c' t e1 e2 ->
+      eq_term c t[/s2/] e1[/s1/] e2[/s2/]
+  | eq_term_by : forall c name t e1 e2,
+      In (name,term_eq_rule c e1 e2 t) l ->
+      eq_term c t e1 e2
+  | eq_term_refl : forall c e t,
+      wf_term c e t ->
+      eq_term c t e e
+  | eq_term_trans : forall c t e1 e12 e2,
+      eq_term c t e1 e12 ->
+      eq_term c t e12 e2 ->
+      eq_term c t e1 e2
+  | eq_term_sym : forall c t e1 e2, eq_term c t e1 e2 -> eq_term c t e2 e1
+  (* Conversion:
+
+c |- e1 = e2 : t 
+               ||
+c |- e1 = e2 : t'
+   *)
+  | eq_term_conv : forall c t t',
+      eq_sort c t t' ->
+      forall e1 e2,
+        eq_term c t e1 e2 ->
+        eq_term c t' e1 e2
+                (*
+  (* TODO: do I want to allow implicit elements in substitutions? *)
+  (* TODO: do I want to define this in terms of eq_args? *)
+  with eq_subst : ctx -> ctx -> subst -> subst -> Prop :=
+  | eq_subst_nil : forall c, eq_subst c [] [] []
+  | eq_subst_cons : forall c c' s1 s2,
+      eq_subst c c' s1 s2 ->
+      forall name t e1 e2,
+        (* assumed because the output ctx is wf: fresh name c' ->*)
+        eq_term c t[/s2/] e1 e2 ->
+        eq_subst c ((name, t)::c') ((name,e1)::s1) ((name,e2)::s2)*)*)
+
+    (*TODO:
+      1. conversion/node id equivalence
+      2. ids for ctxs & types; do I need them?
+         - don't need ctxs since always working in 1 ctx
+         - don't need sorts since the sort is unambiguous up to union-find
+         + should be a relevant lemma in matches
+         - do I need to add sorts to egraph for the above to work?
+     *)
+  Inductive wf_term : ctx -> term -> sort -> positive -> Prop :=
+  | wf_term_by : forall c n s args c' t si i,
+      In (n, term_rule c' args t) l ->
+      wf_args c s c' si ->
+      node_at (ncon n si) i ->
+      wf_term c (con n s) t[/(with_names_from c' s)/] i
+  | wf_term_conv : forall c e t t' i i',
+      (* We add this condition so that we satisfy the assumptions of eq_sort
+         TODO: necessary? not based on current judgment scheme.
+         wf_term c e t should imply wf_sort c t,
+         and eq_sort c t t' should imply wf_sort c t
+
+
+      wf_sort c t -> 
+       *)
+      wf_term c e t i ->
+      wf_sort c t i' ->
+      wf_sort c t' i' ->
+      (*eq_sort c t t' ->*)
+      wf_term c e t' i
+  | wf_term_var : forall c n t i,
+      In (n, t) c ->
+      node_at (nvar n) i ->
+      wf_term c (var n) t i
+  with wf_sort : ctx -> sort -> positive -> Prop :=
+  | wf_sort_by : forall c n s args c' si i,
+      In (n, (sort_rule c' args)) l ->
+      wf_args c s c' si ->
+      node_at (ncon n si) i ->
+      wf_sort c (scon n s) i
+  with wf_args : ctx -> list term -> ctx -> list positive -> Prop :=
+  | wf_args_nil : forall c, wf_args c [] [] []
+  | wf_args_cons : forall c s c' name e t i li,
+      wf_term c e t[/with_names_from c' s/] i ->
+      (* these arguments are last so that proof search unifies existentials
+       from the other arguments first*)
+      wf_args c s c' li ->
+      wf_args c (e::s) ((name,t)::c') (i::li).
+
+
+
+
+
+
+
+
+    
+    (*TODO: change section name?*)
+    Context (c : ctx).
+    Context (wfl : wf_lang l).
+
+
+
+    
+       
+     (*TOOD: replace case_match with this? Copied twice already*)
+     Ltac case_match' :=
+       try lazymatch goal with
+           [ H :  context [ match ?e with
+                            | _ => _
+                            end] |- _ ] => revert H
+         end;
+       case_match.
+    
+  Section Inner.
+
+    Context (proof_result : proof_context).
+    
+    Fixpoint check_args_proof (args : list positive) (c' : ctx) :=
+      match args, c' with
+      | [], [] => Some ([],[])
+      | p::args, (_,t)::c'=>
+          @! let (lhs, rhs) <- check_args_proof args c' in
+            let (term_eq_result e1 e2 t') <?- get p proof_result in
+            (*TODO: use Eqb instance*)
+            let ! sort_eq_dec t[/with_names_from c' rhs/] t' in
+            ret (e1::lhs, e2::rhs)
+      | _,_=> None
+      end.
+
+     Definition check_node (n : node) : option node_result :=
+      match n with
+      | tn_var n =>
+          @! let t <- named_list_lookup_err c n in
+             ret (term_eq_result (var n) (var n) t)
+      | tn_con n s =>
+          @! let r <- named_list_lookup_err l n in
+             match r with
+             | term_rule c' _ t =>
+                 @! let (lhs, rhs) <- check_args_proof s c' in
+                   ret (term_eq_result (con n lhs) (con n rhs)
+                          t[/with_names_from c' rhs/])
+             | term_eq_rule c' e1 e2 t =>
+                 @! let (lhs, rhs) <- check_args_proof s c' in
+                    let lsub := with_names_from c' lhs in
+                    let rsub := with_names_from c' rhs in
+                    ret (term_eq_result e1[/lsub/] e2[/rsub/] t[/rsub/])
+             | _ => None
+             end
+      | tn_trans p0 p1 =>
+          @! let (term_eq_result e1 e2 t) <?- get p0 proof_result in
+             let (term_eq_result e1' e2' t') <?- get p1 proof_result in
+             let ! sort_eq_dec t t' in
+             let ! term_eq_dec e2 e1' in
+             ret (term_eq_result e1 e2' t)
+      | tn_sym p =>
+          @! let (term_eq_result e1 e2 t) <?- get p proof_result in
+             ret (term_eq_result e2 e1 t)
+      | tn_conv p0 p1 =>
+          @! let (sort_eq_result t1 t2) <?- get p0 proof_result in
+             let (term_eq_result e1 e2 t) <?- get p1 proof_result in
+             let ! sort_eq_dec t t1 in
+             ret (term_eq_result e1 e2 t2)
+                 
+      | sn_con n s =>
+          @! let r <- named_list_lookup_err l n in
+             match r with
+             | sort_rule c' _ =>
+                 @! let (lhs, rhs) <- check_args_proof s c' in
+                    ret (sort_eq_result (scon n lhs) (scon n rhs))
+             | sort_eq_rule c' t1 t2 =>
+                 @! let (lhs, rhs) <- check_args_proof s c' in
+                    let lsub := with_names_from c' lhs in
+                    let rsub := with_names_from c' rhs in
+                    ret (sort_eq_result t1[/lsub/] t2[/rsub/])
+             | _ => None
+             end
+      | sn_trans p0 p1 =>
+          @! let (sort_eq_result t1 t2) <?- get p0 proof_result in
+             let (sort_eq_result t1' t2') <?- get p1 proof_result in
+             let ! sort_eq_dec t2 t1' in
+             ret (sort_eq_result t1 t2')
+      | sn_sym p =>
+          @! let (sort_eq_result t1 t2) <?- get p proof_result in
+             ret (sort_eq_result t2 t1)
+      end.
+
+     
+     Definition node_result_sound res :=
+       match res with
+       | term_eq_result e1 e2 t => eq_term l c t e1 e2
+       | sort_eq_result t1 t2 => eq_sort l c t1 t2
+       end.
+
+     (* TODO: move somewhere? *)
+     Definition tree_all {A} (P : A -> Prop) t :=
+       forall n a, get n t = Some a -> P a.
+
+     Context (history_sound : tree_all node_result_sound proof_result).
+
+     
+     Lemma check_args_proof_sound args c' a1 a2
+       : check_args_proof args c' = Some (a1,a2) ->
+         eq_args l c c' a1 a2.
+     Proof.
+       revert c' a1 a2.
+       induction args; destruct c';
+         basic_goal_prep;
+         try congruence;
+         repeat case_match';
+         basic_goal_prep;
+         try congruence;
+         repeat lazymatch goal with
+           | [H : (_,_) = ( _,_) |- _ ] => safe_invert H
+           | [H : Some _ = Some _ |- _ ] => safe_invert H
+          end.
+       - constructor.
+       - constructor; eauto.
+         symmetry in HeqH1.
+         eapply history_sound in HeqH1.
+         exact HeqH1.
+       - safe_invert H.
+       - safe_invert H.
+     Qed.
+     
+     Lemma check_node_sound n res
+       : check_node n = Some res ->
+         node_result_sound res.
+     Proof.
+       destruct n;
+        basic_goal_prep;
+        (*weed out trivial goals for efficiency*)
+        try congruence;
+         repeat case_match';
+        basic_goal_prep;
+        try congruence;
+        repeat lazymatch goal with
+        | [H : default = Some _ |- _ ] => safe_invert H
+        | [H : Some _ = Some _ |- _ ] => safe_invert H
+          end;
+         basic_goal_prep;
+           repeat lazymatch goal with
+           | [H : Some (term_eq_result _ _ _) = _,
+                 hist : tree_all node_result_sound _ |- _] =>
+               symmetry in H;
+               eapply hist in H
+           | [H : Some (sort_eq_result _ _) = _,
+                 hist : tree_all node_result_sound _ |- _] =>
+               symmetry in H;
+               eapply hist in H
+           end; simpl in *; eauto with term lang_core.
+       - constructor; constructor.
+         apply named_list_lookup_err_in; auto.
+       - safe_invert HeqH2; subst.
+         eapply term_con_congruence; eauto.
+         + apply named_list_lookup_err_in; eauto.
+         + eapply check_args_proof_sound; eauto.
+       - eapply eq_term_subst.
+         3: eapply eq_term_by;
+         apply named_list_lookup_err_in; eauto.
+         + apply named_list_lookup_err_in in HeqH.
+           use_rule_in_wf.
+           inversion H; subst.
+           basic_utils_crush.
+         + eapply eq_args_implies_eq_subst.
+           eapply check_args_proof_sound; eauto.
+       - safe_invert HeqH2; subst.
+         eapply sort_con_congruence; eauto.
+         + apply named_list_lookup_err_in; eauto.
+         + eapply check_args_proof_sound; eauto.
+       - eapply eq_sort_subst.
+         3: eapply eq_sort_by;
+         apply named_list_lookup_err_in; eauto.
+         + apply named_list_lookup_err_in in HeqH.
+           use_rule_in_wf.
+           inversion H; subst.
+           basic_utils_crush.
+         + eapply eq_args_implies_eq_subst.
+           eapply check_args_proof_sound; eauto.
+     Qed.
+  End Inner.
+
+  (*TODO: use named_list for pf instead of list?*)
+  Fixpoint check_proof' (p : pf) : option (tree node_result * positive) :=
+    match p with
+    | [] => Some (empty _, 1%positive)
+    | n::p' =>
+        @! let (p_res, next) <- check_proof' p' in
+           let n_res <- check_node p_res n in
+           ret (set next n_res p_res, next + 1)%positive
+    end.
+
+  Definition check_proof (p : pf) : option (term * term * sort) :=
+    @! let (m, next) <- check_proof' p in
+      let (term_eq_result e1 e2 t) <?- get (next - 1)%positive m in
+      ret (e1,e2,t).
+
+      Require Import Lia.
+      Open Scope positive.
+  
+  Lemma check_proof'_fresh' p res next
+    : check_proof' p = Some (res, next) ->
+      forall n', n' >= next ->
+      get n' res = None.
+  Proof.
+    revert res next; induction p;
+      unfold tree_all;
+      basic_goal_prep;
+      repeat lazymatch goal with
+        | [H : default = Some _ |- _ ] => safe_invert H
+        | [H : Some _ = Some _ |- _ ] => safe_invert H
+        end;
+      basic_goal_prep;
+      eauto;
+      repeat case_match';
+      basic_goal_prep;
+      try congruence.
+    safe_invert H.
+    rewrite gso by lia.
+    eapply IHp; eauto; lia.
+  Qed.
+  
+  Lemma check_proof'_fresh p res next
+    : check_proof' p = Some (res, next) ->
+      get next res = None.
+  Proof.
+    intros; eapply check_proof'_fresh'; eauto; lia.
+  Qed.
+    
+  Lemma check_proof'_sound p res next
+    : check_proof' p = Some (res, next) ->
+      tree_all node_result_sound res.
+  Proof.
+    revert res next; induction p;
+      unfold tree_all;
+      basic_goal_prep;
+        repeat lazymatch goal with
+        | [H : default = Some _ |- _ ] => safe_invert H
+        | [H : Some _ = Some _ |- _ ] => safe_invert H
+          end;
+      basic_goal_prep;
+      eauto using check_node_sound;
+    repeat case_match';
+      basic_goal_prep;
+      try congruence.
+    safe_invert H; simpl.
+    safe_invert HeqH0.
+    destruct (Pos.eq_dec n p0).
+    {
+      subst.
+      rewrite gss in H0.
+      safe_invert H0.
+      eapply check_node_sound; eauto.      
+    }
+    rewrite gso in H0; eauto.
+    eapply IHp; eauto.
+  Qed.
+
+  Theorem check_proof_sound p e1 e2 t
+    : check_proof p = Some (e1,e2,t) ->
+      eq_term l c t e1 e2.
+  Proof.
+    unfold check_proof.
+    remember (check_proof' p) as check.
+    destruct check; simpl; try congruence.
+    destruct p0; simpl; try congruence.
+    repeat case_match;
+      basic_goal_prep;
+        repeat lazymatch goal with
+        | [H : default = Some _ |- _ ] => safe_invert H
+        | [H : Some _ = Some _ |- _ ] => safe_invert H
+          end;
+      try congruence.
+    symmetry in Heqcheck.
+    apply check_proof'_sound in Heqcheck.
+    simpl in *.
+    symmetry in HeqH.
+    specialize (Heqcheck _ _ HeqH).
+    eauto.
+  Qed.
+   *)
+
+  End WithLang.
+
+End WithVar.
